Challenge/Modexp/Submission/Proofs/Fast/CiosCachedPrograms.lean
@@ -85,7 +85,12 @@ def l2Program (w : Fin 33) (x tl ts : UInt256) : List Instr :=
     macProductProgram) ++ macFinishProgram tl ts
 
 def entryProgram : List Instr :=
-  [.op .JUMPDEST,
+  [
+   .op .JUMPDEST,
+   .push 2 9440,
+   .op .MLOAD,
+   .push 2 9376,
+   .op .MLOAD,
    .push 2 9408,
    .op .MLOAD,
    .op .MLOAD,
@@ -98,17 +103,19 @@ def entryProgram : List Instr :=
    .push 1 150,
    .op .MUL,
    .op (.Dup ⟨0, by decide⟩),
-   .push 2 4229,
+   .push 2 4239,
    .op .ADD,
    .op (.Swap ⟨0, by decide⟩),
-   .push 2 4570,
+   .push 2 4574,
    .op .ADD,
    .op (.Swap ⟨3, by decide⟩),
    .op (.Swap ⟨4, by decide⟩),
+   .op (.Swap ⟨6, by decide⟩),
    .push 0 0,
    .op .NOT,
    .op (.Swap ⟨3, by decide⟩),
    .op (.Swap ⟨5, by decide⟩),
+   .op (.Swap ⟨6, by decide⟩),
    .push 2 9344,
    .op .MLOAD,
    .op (.Dup ⟨0, by decide⟩),
@@ -138,7 +145,8 @@ def outProgram : List Instr :=
    .push 0 0]
 
 def midProgram : List Instr :=
-  [.op (.Dup ⟨0, by decide⟩),
+  [
+   .op (.Dup ⟨0, by decide⟩),
    .push 2 8224,
    .op .MLOAD,
    .op .ADD,
@@ -148,12 +156,10 @@ def midProgram : List Instr :=
    .op .LT,
    .push 2 8192,
    .op .MSTORE,
-   .push 2 9440,
-   .op .MLOAD,
+   .op (.Dup ⟨10, by decide⟩),
    .op .MLOAD,
    .op (.Dup ⟨0, by decide⟩),
-   .push 2 9376,
-   .op .MLOAD,
+   .op (.Dup ⟨11, by decide⟩),
    .op .MUL,
    .op (.Swap ⟨0, by decide⟩),
    .op (.Dup ⟨10, by decide⟩),
@@ -169,7 +175,8 @@ def midProgram : List Instr :=
    .op .ADD]
 
 def tailProgram : List Instr :=
-  [.op (.Swap ⟨1, by decide⟩),
+  [
+   .op (.Swap ⟨1, by decide⟩),
    .op .POP,
    .op .POP,
    .op (.Dup ⟨0, by decide⟩),
@@ -190,8 +197,10 @@ def tailProgram : List Instr :=
    .op (.Dup ⟨2, by decide⟩),
    .op (.Dup ⟨1, by decide⟩),
    .op .GT,
-   .push 2 4223,
+   .push 2 4233,
    .op .JUMPI,
+   .op .POP,
+   .op .POP,
    .op .POP,
    .op .POP,
    .op .POP,
